Define a synonym for [Cursor 32]
After     | File Name               | Before    || Change
------------------------------------------------------------
17m53.40s | Total                   | 18m42.90s || -0m49.50s
------------------------------------------------------------
1m14.35s  | x86/globals             | 1m28.68s  || -0m14.33s
0m53.86s  | x86/call                | 1m04.21s  || -0m10.34s
0m28.56s  | x86/matcher             | 0m38.74s  || -0m10.18s
3m44.02s  | x86/instrrules          | 3m50.23s  || -0m06.20s
0m28.72s  | x86/listproof           | 0m33.85s  || -0m05.13s
0m23.36s  | x86/inlinealloc         | 0m27.67s  || -0m04.31s
0m28.56s  | x86/cfuncspec           | 0m32.30s  || -0m03.73s
0m23.14s  | x86/mulc                | 0m27.12s  || -0m03.98s
0m19.59s  | x86/win/pecoff          | 0m16.47s  || +0m03.12s
0m18.30s  | x86/wrapalloc           | 0m21.97s  || -0m03.66s
0m17.26s  | x86/lifeimp             | 0m20.85s  || -0m03.58s
0m18.42s  | x86/programassemcorrect | 0m15.63s  || +0m02.79s
0m16.63s  | x86/main                | 0m18.68s  || -0m02.05s
0m15.21s  | bitsopsprops            | 0m13.16s  || +0m02.05s
0m14.59s  | x86/specexamples        | 0m16.80s  || -0m02.21s
0m14.45s  | x86/screenproof         | 0m17.25s  || -0m02.80s
0m13.88s  | x86/imp                 | 0m16.79s  || -0m02.90s
0m10.83s  | x86/cstringimp          | 0m13.51s  || -0m02.67s
0m09.70s  | x86/xorswap             | 0m11.96s  || -0m02.26s
0m15.20s  | x86/instrcodec          | 0m14.04s  || +0m01.16s
0m15.12s  | spec                    | 0m13.20s  || +0m01.92s
0m12.42s  | triple                  | 0m11.34s  || +0m01.08s
0m10.39s  | codec                   | 0m09.18s  || +0m01.21s
0m09.67s  | regex                   | 0m08.14s  || +0m01.52s
0m09.41s  | spectac                 | 0m07.87s  || +0m01.54s
0m08.70s  | septac                  | 0m07.09s  || +0m01.60s
0m07.84s  | safe                    | 0m06.55s  || +0m01.29s
0m07.35s  | x86/gcdex               | 0m08.98s  || -0m01.63s
0m07.02s  | codecregex              | 0m05.96s  || +0m01.05s
0m05.75s  | x86/eval                | 0m04.69s  || +0m01.05s
0m21.32s  | pointsto                | 0m22.21s  || -0m00.89s
0m18.78s  | x86/macros              | 0m19.36s  || -0m00.57s
0m11.90s  | bitstest                | 0m11.75s  || +0m00.15s
0m09.97s  | x86/program             | 0m09.40s  || +0m00.57s
0m07.46s  | x86/basic               | 0m07.51s  || -0m00.04s
0m06.50s  | SPred                   | 0m05.99s  || +0m00.50s
0m06.42s  | x86/fact                | 0m07.18s  || -0m00.75s
0m06.33s  | x86/testrun             | 0m07.24s  || -0m00.91s
0m06.26s  | x86/cfunc               | 0m07.03s  || -0m00.77s
0m06.22s  | x86/examples            | 0m07.12s  || -0m00.90s
0m06.21s  | x86/listspec            | 0m07.13s  || -0m00.92s
0m06.19s  | x86/screenimp           | 0m06.81s  || -0m00.61s
0m06.16s  | x86/listimp             | 0m06.80s  || -0m00.63s
0m06.13s  | x86/basicprog           | 0m06.32s  || -0m00.19s
0m06.13s  | x86/programeq           | 0m05.52s  || +0m00.61s
0m06.04s  | x86/programassem        | 0m05.44s  || +0m00.59s
0m05.99s  | x86/entry               | 0m06.71s  || -0m00.71s
0m05.82s  | x86/screenspec          | 0m05.95s  || -0m00.12s
0m05.75s  | pmapprops               | 0m04.91s  || +0m00.83s
0m05.74s  | x86/encdechelp          | 0m04.94s  || +0m00.79s
0m05.71s  | roundtrip               | 0m05.80s  || -0m00.08s
0m05.70s  | bitsprops               | 0m05.01s  || +0m00.69s
0m05.63s  | bitscodec               | 0m04.73s  || +0m00.89s
0m05.48s  | bitreader               | 0m05.90s  || -0m00.41s
0m04.99s  | x86/reg                 | 0m04.36s  || +0m00.62s
0m04.94s  | x86/ioaction            | 0m04.25s  || +0m00.69s
0m04.92s  | x86/step                | 0m04.60s  || +0m00.32s
0m04.91s  | x86/procstatemonad      | 0m04.37s  || +0m00.54s
0m04.76s  | bitsrep                 | 0m03.96s  || +0m00.79s
0m04.72s  | writer                  | 0m04.60s  || +0m00.12s
0m04.69s  | pmap                    | 0m03.96s  || +0m00.73s
0m04.67s  | x86/regstate            | 0m04.12s  || +0m00.54s
0m04.67s  | x86/procstate           | 0m04.43s  || +0m00.24s
0m04.66s  | x86/flags               | 0m04.12s  || +0m00.54s
0m04.62s  | enc                     | 0m04.09s  || +0m00.53s
0m04.60s  | x86/instr               | 0m04.11s  || +0m00.48s
0m04.48s  | cursor                  | 0m04.59s  || -0m00.10s
0m04.47s  | bitsops                 | 0m03.91s  || +0m00.55s
0m04.45s  | nathelp                 | 0m03.70s  || +0m00.75s
0m04.40s  | reader                  | 0m04.36s  || +0m00.04s
0m04.36s  | charge/iltac            | 0m03.85s  || +0m00.51s
0m04.31s  | x86/mem                 | 0m04.34s  || -0m00.03s
0m04.15s  | x86/instrsyntax         | 0m03.96s  || +0m00.19s
0m03.41s  | charge/ilogic           | 0m02.76s  || +0m00.65s
0m03.08s  | charge/bilogic          | 0m02.80s  || +0m00.28s
0m03.07s  | charge/sepalg           | 0m02.60s  || +0m00.46s
0m02.94s  | sparsefun               | 0m02.36s  || +0m00.58s
0m02.91s  | tuplehelp               | 0m02.46s  || +0m00.45s
0m02.91s  | charge/later            | 0m02.62s  || +0m00.29s
0m02.79s  | cast                    | 0m02.22s  || +0m00.56s
0m02.73s  | monadinst               | 0m02.29s  || +0m00.43s
0m02.56s  | monad                   | 0m02.07s  || +0m00.49s
0m02.55s  | cstring                 | 0m02.11s  || +0m00.43s
0m02.43s  | emb                     | 0m02.04s  || +0m00.39s
0m02.38s  | ilogicss                | 0m02.62s  || -0m00.24s
0m02.23s  | x86/exn                 | 0m01.90s  || +0m00.33s
0m01.38s  | charge/CSetoid          | 0m01.05s  || +0m00.32s
0m01.18s  | pfun                    | 0m00.94s  || +0m00.24s
0m00.48s  | common_tactics          | 0m00.37s  || +0m00.10s
0m00.46s  | update                  | 0m00.35s  || +0m00.11s

src/cursor.v
@@ -312,6 +312,23 @@ End Cursors.
 
 Coercion mkCursor : BITS >-> Cursor.
 
+(** Convenience definitions for various sizes of cursor *)
+(*Definition NIBBLECursor := Cursor 4.
+Definition BYTECursor   := Cursor 8.
+Definition WORDCursor   := Cursor 16.*)
+Definition DWORDCursor  := Cursor 32.
+(*Definition QWORDCursor  := Cursor 64.
+Definition DWORDorBYTECursor (d: bool) := Cursor (if d then 32 else 8).*)
+
+(*Coercion mkNIBBLECursor (x: NIBBLE) : NIBBLECursor := mkCursor x.
+Coercion mkBYTECursor   (x: BYTE)   : BYTECursor   := mkCursor x.
+Coercion mkWORDCursor   (x: WORD)   : WORDCursor   := mkCursor x.
+Coercion mkDWORDCursor  (x: DWORD)  : DWORDCursor  := mkCursor x.
+Coercion mkQWORDCursor  (x: QWORD)  : QWORDCursor  := mkCursor x.
+Coercion mkDWORDorBYTECursor d (x: DWORDorBYTE d) : DWORDorBYTECursor d := mkCursor x.*)
+
+Identity Coercion DWORDCursortoCursor32 : DWORDCursor >-> Cursor.
+
 Lemma nextCat n1 n2 (p:BITS n1) m : m < (2^n2).-1 ->
   next (p ## fromNat (n:=n2) m) = p ## #(m.+1).
 Proof. move => LT.
@@ -427,4 +444,3 @@ Section CursorCanonicals.
   Definition Cursor_finMixin := Eval hnf in CanFinMixin cursor_optionC.
   Canonical Structure Cursor_finType := Eval hnf in FinType _ Cursor_finMixin.
 End CursorCanonicals.
-
